## Conjunto de Premissas %% fold %%

## Enunciado
- Solve this differential equation:
$$\frac{dy}{dx} - x - x^2 = 0$$
where
$$y(0) = 1$$

## Desenvolvimento %% fold %%

1. Multiply both sides by $dx$:
$$dy - x\,dx - x^2\,dx = 0$$

2. Separate $x$ and $y$ terms on different sides of the equal sign:
$$dy = x\,dx + x^2\,dx$$

3. Then integrate to get
$$y = \frac{x^2}{2} + \frac{x^3}{3} + c$$

4. Apply the initial conditions to find that $c = 1$

5. Tada! The solution is
$$y = \frac{x^2}{2} + \frac{x^3}{3} + 1$$


## Respostas %% fold %%
$$y = \frac{x^2}{2} + \frac{x^3}{3} + 1$$
